intermediate/README.md
@@ -2,17 +2,16 @@
 
 ## Overview
 
-The goal is to connect the high-level math proof (in the top-level directory) to an implementation that can be run on a machine (in the `low-level` sub-directory). We will do this by showing that the low-level code simulates the high-level formalism, via a series intermediate steps that reduce proof complexity. The stages of moving from the high-level specification to the low-level code are shown below.
+The goal is to connect the high-level math proof (in the 'high' directory) to an implementation that can be run on a machine (in the `low` directory). We will do this by showing that the low-level code simulates the high-level formalism, via a single intermediate step that reduce proof complexity. The stages of moving from the high-level specification to the low-level code are shown below.
 1. **Spec** The high-level model where the proof of correctness is given. The store is modelled as a functional map from keys to values.
-2. **InterSC** Intermediate representation with Slots and runtime Checks for duplicate entries. The store is modelled as a sequence of (key, value, add_method) triples. Log entries record "slot_id"s used to index into the sequence; adds, gets, and puts also include argument keys. At every add, it performs a search through the entire store to see if a key has been added previously.
-3. **InterS** Intermediate representation with Slots, without inefficient checks for existing keys. Stores extra information in merkle nodes to determine if a key is already present, but relies on hash validation to eventually find the case where a key has been added multiple times using Blum.
-4. **Low**  Low* implementation. Same as **InterS** except it uses C-compatible data types (e.g. Buffer instead of Seq).
+2. **Inter** The store is modelled as a sequence of (key, value, add_method) entries, with two extra bits to determine if a key has been added to the store via Merkle. Log entries record "slot_id"s used to index into the sequence; adds, gets, and puts also include argument keys.
+3. **Low**  Low* implementation. Same as **Inter** except it uses C-compatible data types (e.g. Buffer instead of Seq).
 
-**TODO:** All the levels of the current formalization assume a single epoch (i.e. one "offline" verification step). The Low* code should be modified to support multiple epochs, and we should add another layer after **InterS** (e.g. **InterE**) that introduces epochs.
+**TODO:** All the levels of the current formalization assume a single epoch (i.e. one "offline" verification step). The Low* code should be modified to support multiple epochs, and we should add another layer after **Inter** (e.g. **InterE**) that introduces epochs.
 
 ## Log Types
 
-In the intermediate levels above, we use a three different types of logs. The **Spec** level uses the following definition of log entries (in Veritas.Verifier).
+The **Spec** level uses the following definition of log entries (in Veritas.Verifier).
 ```
 type vlog_entry =
   | Get: k:data_key -> v:data_value -> vlog_entry
@@ -23,7 +22,7 @@ type vlog_entry =
   | EvictB: k:key -> t:timestamp -> vlog_entry
   | EvictBM: k:key -> k':merkle_key -> t:timestamp -> vlog_entry
 ```
-The **InterSC** and **InterS** levels use log entries with "slot ids" (in Veritas.Intermediate.Logs).
+The **Inter** level uses log entries with "slot ids" (in Veritas.Intermediate.Logs).
 ```
 type logS_entry =
   | Get_S: s:slot_id -> k:data_key -> v:data_value -> logS_entry
@@ -36,7 +35,7 @@ type logS_entry =
 ```
 The **Low** level also uses a log with slot ids, but additionally uses C-compatible data types (TODO).
 
-We call logs with keys `logK`, logs with slots `logK`, and low-level logs `logL`. We provide a function `logS_to_logK : logS -> logK` that converts from a `logS` to a `logK` using the **InterSC** level verifier. Assume we also provide a `logL_to_logS` function, which should e a simple conversion.
+We call logs with keys `logK`, logs with slots `logK`, and low-level logs `logL`. We provide a function `logS_to_logK : logS -> logK` that converts from a `logS` to a `logK` using the **InterSC** level verifier. Assume we also provide a `logL_to_logS` function, which should be a simple conversion.
 
 ## Proof Structure
 
@@ -47,19 +46,12 @@ let lemma_verifier_correct (gl: VG.hash_verifiable_log { ~ (seq_consistent (to_s
 ```
 In English: if a global log is verifiable then if a (i.e. the events are sequentially consistent, modulo hash collisions). *Sequential consistency* says that there exists an ordering among the different thread's events such that any "Get k" reads the most recent value written to k.
 
-The property we want for **Low** is identical: If a log is verifiable, then any "Get s k" reads the most recent value written to k. (Intermediate level verification will also check that k is stored at slot s, but this can be ignore in the final statement of correctness.)
+The property we want for **Low** is identical: If a log is verifiable, then any "Get s k" reads the most recent value written to k. (Intermediate level verification will also check that k is stored at slot s, but this can be ignored in the final statement of correctness.)
 
-The property above for **Spec** implies the property we want for **Low** *provided* that we can prove the following: If **Low** says `log` is verifiable
-* then **InterS** says `log2` is verifiable where `log2=logL_to_logS(log)`
-* then **InterSC** says `log2` is verifiable
-* then **Spec** says the `log3` is verifiable where `log3=logS_to_logK(log2)`
-
-Note that may be possible to prove equality rather than implication for some of these levels. For example, `InterS.verifiable log2 = InterSC.verifiable log2`.
+[TODO]
 
 ## Directory Contents
 
 * Veritas.Intermediate.Logs.fst - A definition of logs with slots (logS) and wrappers around high- and low-level logs (logK and logL) 
-* Veritas.Intermediate.StoreSC.fst(i) - Functions for manipulating a sequence of (key, value, add_method) triples. Used in VerifySC.
-* Veritas.Intermediate.VerifySC.fst(i) - Description of **InterSC** verification and proof that this simulates **Spec** verification.
-* Veritas.Intermediate.StoreS.fst(i) - Functions for manipulating a sequence of (key, value, add_method, l_child_in_store, r_child_in_store) records. Used in VerifyS.
-* Veritas.Intermediate.VerifyS.fst(i) - Description of **InterS** verification and proof that this simulates **InterSC** verification.
+* Veritas.Intermediate.Store.fst(i) - Functions for manipulating a sequence of (key, value, add_method, l-bit, r-bit) records. Used in Intermediate.Verify.
+* Veritas.Intermediate.Verify.fst(i) - Description of **Inter** verification and proof that this simulates **Spec** verification.
